grammatik/Grammatik.lean
@@ -324,3 +324,4 @@ import Grammatik.Zielsatz.Schwach
 import Grammatik.Speichermodell.Zeuge
 import Grammatik.Speichermodell.Atomar
 import Grammatik.Speichermodell.AtomarZeuge
+import Grammatik.Speichermodell.Zaehler
